Use downviews for X64.Memory

vale/code/arch/x64/Interop.fsti
@@ -4,6 +4,7 @@ module HS = FStar.Monotonic.HyperStack
 module HH = FStar.Monotonic.HyperHeap
 module MB = LowStar.Monotonic.Buffer
 module M = LowStar.Modifies
+module DV = LowStar.BufferView.Down
 
 open Opaque_s
 open Interop.Base
@@ -14,7 +15,7 @@ open X64.Bytes_Semantics
 let op_String_Access = Map.sel
 let op_String_Assignment = Map.upd
 
-let disjoint (ptr1 ptr2:b8) = MB.loc_disjoint (MB.loc_buffer ptr1.b) (MB.loc_buffer ptr2.b)
+let disjoint (ptr1 ptr2:b8) = MB.loc_disjoint (MB.loc_buffer ptr1.bsrc) (MB.loc_buffer ptr2.bsrc)
 
 let valid_addr (mem:mem) (x:int) = Set.mem x (addrs_set mem)
 
@@ -22,14 +23,14 @@ val addrs_set_lemma (mem:mem) (x:int)
   : Lemma (let addrs = addrs_of_mem mem in
            let ptrs = ptrs_of_mem mem in
            valid_addr mem x <==>
-           (exists (b:b8{List.memP b ptrs}).{:pattern (addrs b)} addrs b <= x /\ x < addrs b + MB.length b.b))
+           (exists (b:b8{List.memP b ptrs}).{:pattern (addrs b)} addrs b <= x /\ x < addrs b + DV.length (get_downview b.bsrc)))
           [SMTPat (Set.mem x (addrs_set mem))]
   
 let addrs_set_mem (mem:mem) (a:b8) (i:int)
   : Lemma
     (requires (let ptrs = ptrs_of_mem mem in
                let addrs = addrs_of_mem mem in
-               List.memP a ptrs /\ i >= addrs a /\ i < addrs a + MB.length a.b))
+               List.memP a ptrs /\ i >= addrs a /\ i < addrs a + DV.length (get_downview a.bsrc)))
     (ensures valid_addr mem i)
   = ()
   
@@ -50,8 +51,8 @@ val same_unspecified_down:
          heap1.[i] == heap2.[i])
 
 let get_seq_heap (heap:heap) (addrs:addr_map) (b:b8) 
-  : GTot (Seq.lseq UInt8.t (MB.length b.b)) 
-  = let length = MB.length b.b in
+  : GTot (Seq.lseq UInt8.t (DV.length (get_downview b.bsrc))) 
+  = let length = DV.length (get_downview b.bsrc) in
     let contents (i:nat{i < length}) = UInt8.uint_to_t heap.[addrs b + i] in
     Seq.init length contents
 
@@ -68,13 +69,13 @@ val up_down_identity (mem:mem)
       (requires (forall x. not (Map.contains heap x) ==> Map.sel heap x == Map.sel (down_mem mem) x))
       (ensures (down_mem (up_mem heap mem) == heap))
 
-val update_buffer_up_mem
-      (mem:mem)
-      (b:b8{List.memP b (ptrs_of_mem mem)})
-      (heap1:heap{correct_down mem heap1})
-      (heap2:heap{Set.equal (Map.domain heap1) (Map.domain heap2)})
- : Lemma
-      (requires (forall x. x < addrs_of_mem mem b \/ x >= addrs_of_mem mem b + MB.length b.b
-        ==> heap1.[x] == heap2.[x]))
-      (ensures hs_of_mem (up_mem heap2 mem) ==
-               MB.g_upd_seq b.b (get_seq_heap heap2 (addrs_of_mem mem) b) (hs_of_mem mem))
+// val update_buffer_up_mem
+//       (mem:mem)
+//       (b:b8{List.memP b (ptrs_of_mem mem)})
+//       (heap1:heap{correct_down mem heap1})
+//       (heap2:heap{Set.equal (Map.domain heap1) (Map.domain heap2)})
+//  : Lemma
+//       (requires (forall x. x < addrs_of_mem mem b \/ x >= addrs_of_mem mem b + DV.length (get_downview b.bsrc)
+//         ==> heap1.[x] == heap2.[x]))
+//       (ensures hs_of_mem (up_mem heap2 mem) ==
+//                DV.upd_seq (hs_of_mem mem) (get_downview b.bsrc) (get_seq_heap heap2 (addrs_of_mem mem) b))
